1) redesigned computation by the undef values ideas, proved that const2GV is not stuck 2) supported LLVM names with escaped chars 3) recovered interpreter regression, which is failed from version 2964, from then, the constant null's type is restricted to be pointer types syntactially, while interpreter was not consistent with this invariant. 4) A known problem of OCaml llvm bindings, the translation of 129.compress outputs a strange '^@' where it should print '0', this could be by some illegal memory access from ocaml-llvm bindings.
git-svn-id: https://webdav.seas.upenn.edu/svn/sol/vol@2978 eef5ea85-cc2e-0410-bd84-0fae1f012da8

src/ssa/genericvalues.v
@@ -45,6 +45,7 @@ end.
 
 Definition uninits (n:nat) : GenericValue := 
    Coqlib.list_repeat n (Vundef, Mint 7).
+Definition gundef := uninits 1.
 Definition GV2val (TD:TargetData) (gv:GenericValue) : option val :=
 match gv with
 | (v,c)::nil => Some v
@@ -314,45 +315,57 @@ match lgv with
 end.
 
 (* FIXME : bounds check *)
-Definition extractGenericValue (TD:TargetData)(t:typ) (gv : GenericValue) 
+Definition extractGenericValue (TD:TargetData) (t:typ) (gv : GenericValue) 
   (cidxs : list_const) : option GenericValue :=
 match (intConsts2Nats TD cidxs) with
-| None => None 
+| None => Some gundef
 | Some idxs =>
   match (mgetoffset TD t idxs) with
-  | Some o => mget TD gv o t
-  | None => None
+  | Some o => match mget TD gv o t with 
+              | Some gv' => Some gv'
+              | None => Some gundef
+              end
+  | None => Some gundef
   end
 end.
 
 Definition insertGenericValue (TD:TargetData) (t:typ) (gv:GenericValue)
   (cidxs:list_const) (t0:typ) (gv0:GenericValue) : option GenericValue :=
 match (intConsts2Nats TD cidxs) with
-| None => None 
+| None => Some gundef
 | Some idxs =>
   match (mgetoffset TD t idxs) with
-  | Some o => mset TD gv o t0 gv0
-  | None => None
+  | Some o => match (mset TD gv o t0 gv0) with
+              | Some gv' => Some gv'
+              | None => Some gundef
+              end
+  | None => Some gundef
   end
 end.
 
 Definition mtrunc (TD:TargetData) (op:truncop) (t1:typ) (gv1:GenericValue) 
   (t2:typ) : option GenericValue :=
-match (GV2val TD gv1, t1, t2) with
-| (Some (Vint wz1 i1), typ_int sz1, typ_int sz2) =>
-  if eq_nat_dec wz1 sz1
-  then Some (val2GV TD (Val.trunc (Vint wz1 i1) sz2) (Mint sz2))
-  else None
-| (Some (Vfloat f), typ_floatpoint fp1, typ_floatpoint fp2) =>
-  if floating_point_order fp2 fp1 
-  then 
-    match fp2 with
-    | fp_float => Some (val2GV TD (Val.ftrunc (Vfloat f)) Mfloat32)
-    | fp_double => Some (val2GV TD (Val.ftrunc (Vfloat f)) Mfloat64)
-    | _ => None (*FIXME: not supported 80 and 128 yet. *)
+match GV2val TD gv1 with
+| Some (Vint wz1 i1) =>
+    match (t1, t2) with
+    | (typ_int sz1, typ_int sz2) =>
+        Some (val2GV TD (Val.trunc (Vint wz1 i1) sz2) (Mint sz2))
+    | _ => Some gundef
     end
-  else None
-| (_, _, _) => None
+| Some (Vfloat f) =>
+    match (t1, t2) with
+    | (typ_floatpoint fp1, typ_floatpoint fp2) =>
+        if floating_point_order fp2 fp1 
+        then 
+          match fp2 with
+          | fp_float => Some (val2GV TD (Val.ftrunc (Vfloat f)) Mfloat32)
+          | fp_double => Some (val2GV TD (Val.ftrunc (Vfloat f)) Mfloat64)
+          | _ => None (* FIXME: not supported 80 and 128 yet. *)
+          end
+        else None
+    | _ => Some gundef
+    end
+| _ => Some gundef
 end.
 
 Definition mbop (TD:TargetData) (op:bop) (bsz:sz) (gv1 gv2:GenericValue) 
@@ -390,8 +403,8 @@ match (GV2val TD gv1, GV2val TD gv2) with
      | bop_xor => 
          Some (val2GV TD (Val.xor (Vint wz1 i1) (Vint wz2 i2)) (Mint (bsz'-1)))
      end
-  else None
-| _ => None
+  else Some gundef
+| _ => Some gundef
 end.
 
 Definition mfbop (TD:TargetData) (op:fbop) (fp:floating_point) 
@@ -409,10 +422,27 @@ match (GV2val TD gv1, GV2val TD gv2) with
   match fp with
   | fp_float => Some (val2GV TD v Mfloat32)
   | fp_double => Some (val2GV TD v Mfloat64)
-  | _ => None (*FIXME: not supported 80 and 128 yet. *)
+  | _ => None (* FIXME: not supported 80 and 128 yet. *)
   end
-| _ => None
+| _ => Some gundef
 end.
+
+Definition mptrtoint (TD:TargetData) (M:mem) (gv1:GenericValue) (sz2:nat)
+ : option GenericValue :=
+    match GV2val TD gv1 with
+    | Some (Vptr b1 ofs1) =>
+        match Mem.ptr2int M b1 0 with
+        | Some z => 
+            Some (val2GV TD 
+                   (Vint sz2 (Int.repr sz2 (z + Int.signed 31 ofs1))) 
+                   (Mint sz2))
+        | None => Some (val2GV TD (Vint sz2 (Int.zero sz2)) (Mint sz2))
+        end
+    | Some (Vinttoptr i) => 
+        Some (val2GV TD (Vint sz2 (Int.repr sz2 (Int.unsigned 31 i))) (Mint sz2))
+    | _ => Some gundef
+    end.
+
 
 Definition mcast (TD:TargetData) (M:mem) (op:castop) (t1:typ) (gv1:GenericValue)
   (t2:typ) : option GenericValue :=
@@ -427,26 +457,13 @@ match op with
         | None => 
             Some (ptr2GV TD (Vinttoptr (Int.repr 31 (Int.unsigned wz1 i1))))
         end
-    | _ => None
+    | _ => Some gundef
     end
   | _ => None
   end
 | castop_ptrtoint =>
   match (t1, t2) with
-  | (typ_pointer _, typ_int sz2) => 
-    match GV2val TD gv1 with
-    | Some (Vptr b1 ofs1) =>
-        match Mem.ptr2int M b1 0 with
-        | Some z => 
-            Some (val2GV TD 
-                   (Vint sz2 (Int.repr sz2 (z + Int.signed 31 ofs1))) 
-                   (Mint sz2))
-        | None => Some (val2GV TD (Vint sz2 (Int.zero sz2)) (Mint sz2))
-        end
-    | Some (Vinttoptr i) => 
-        Some (val2GV TD (Vint sz2 (Int.repr sz2 (Int.unsigned 31 i))) (Mint sz2))
-    | _ => None
-    end
+  | (typ_pointer _, typ_int sz2) => mptrtoint TD M gv1 sz2
   | _ => None
   end
 | castop_bitcase =>
@@ -468,9 +485,9 @@ match (t1, t2) with
                         (Mint (Size.to_nat sz2-1)))
      | extop_s => Some (val2GV TD (Val.sign_ext (Size.to_Z sz2) (Vint wz1 i1)) 
                         (Mint (Size.to_nat sz2-1)))
-     | _ => None
+     | _ => Some gundef
      end
-   | _ => None
+   | _ => Some gundef
    end
 | (typ_floatpoint fp1, typ_floatpoint fp2) => 
   if floating_point_order fp1 fp2 
@@ -481,16 +498,13 @@ match (t1, t2) with
       | extop_fp => Some gv1
       | _ => None
       end
-    | _ => None
+    | _ => Some gundef
     end
   else None
 | (_, _) => None
 end.
 
-Definition micmp (TD:TargetData) (c:cond) (t:typ) (gv1 gv2:GenericValue) 
-  : option GenericValue :=
-match t with
-| typ_int sz =>
+Definition micmp_int TD c gv1 gv2 : option GenericValue :=
   match (GV2val TD gv1, GV2val TD gv2) with
   | (Some (Vint wz1 i1), Some (Vint wz2 i2)) => 
      match c with
@@ -515,8 +529,19 @@ match t with
      | cond_sle => 
          Some (val2GV TD (Val.cmp Cle (Vint wz1 i1) (Vint wz2 i2)) (Mint 0))
      end
-  | _ => None
-  end  
+  | _ => Some gundef
+  end.  
+
+Definition micmp (TD:TargetData) (M:mem) (c:cond) (t:typ) (gv1 gv2:GenericValue) 
+  : option GenericValue :=
+match t with
+| typ_int sz => micmp_int TD c gv1 gv2
+| typ_pointer _ => 
+  match (mptrtoint TD M gv1 Size.ThirtyTwo, mptrtoint TD M gv2 Size.ThirtyTwo)
+    with
+  | (Some gv1', Some gv2') => micmp_int TD c gv1' gv2'
+  | _ => Some gundef
+  end
 | _ => None
 end.
 
@@ -560,22 +585,7 @@ match (GV2val TD gv1, GV2val TD gv2) with
    | fp_double => ov
    | _ => None (*FIXME: not supported 80 and 128 yet. *)
    end  
-| _ => None
-end.
-
-Definition GEP (TD:TargetData) (t:typ) (ma:GenericValue) 
-  (vidxs:list GenericValue) (inbounds:bool) : option GenericValue :=
-match GV2ptr TD (getPointerSize TD) ma with
-| Some ptr =>
-  match GVs2Nats TD vidxs with
-  | None => None 
-  | Some idxs => 
-    match (mgep TD t ptr idxs) with
-    | Some ptr0 => Some (ptr2GV TD ptr0)
-    | None => None
-    end
-  end
-| None => None
+| _ => Some gundef
 end.
 
 (**************************************)
@@ -587,7 +597,7 @@ match n with
 | S n' => gv++repeatGV gv n'
 end.
 
-Fixpoint _zeroconst2GV (TD:TargetData) (t:typ) : option GenericValue :=
+Fixpoint zeroconst2GV (TD:TargetData) (t:typ) : option GenericValue :=
 match t with
 | typ_int sz => 
   let wz := (Size.to_nat sz) - 1 in
@@ -596,13 +606,13 @@ match t with
   match fp with
   | fp_float => Some (val2GV TD (Vfloat Float.zero) Mfloat32)
   | fp_double => Some (val2GV TD (Vfloat Float.zero) Mfloat64)
-  | _ => None (*FIXME: not supported 80 and 128 yet. *)
+  | _ => None (* FIXME: not supported 80 and 128 yet. *)
   end
 | typ_void => None          
 | typ_label => None                     
 | typ_metadata => None                
 | typ_array sz t => 
-  match _zeroconst2GV TD t with
+  match zeroconst2GV TD t with
   | Some gv0 =>
     match (getTypeStoreSize TD t, getTypeAllocSize TD t) with
     | (Some ssz, Some asz) => 
@@ -613,7 +623,7 @@ match t with
   | _ => None
   end
 | typ_struct ts => 
-  match _list_typ_zerostruct2GV TD ts with
+  match zeroconsts2GV TD ts with
   | Some (gv0, tsz) => 
       match getTypeAllocSize TD t with
       | Some asz => 
@@ -630,12 +640,12 @@ match t with
 | typ_opaque => None
 | typ_namedt _ => None (*FIXME: Can zeroconstant be of named type? How about termination. *)
 end             
-with _list_typ_zerostruct2GV (TD:TargetData) (lt:list_typ) 
+with zeroconsts2GV (TD:TargetData) (lt:list_typ) 
   : option (GenericValue * nat) := 
 match lt with
 | Nil_list_typ => Some (nil, 0)
 | Cons_list_typ t lt' =>
-  match (_list_typ_zerostruct2GV TD lt', _zeroconst2GV TD t) with
+  match (zeroconsts2GV TD lt', zeroconst2GV TD t) with
   | (Some (gv, tsz), Some gv0) =>
        match (getTypeStoreSize TD t, getTypeAllocSize TD t) with
        | (Some ssz, Some asz) => Some (gv++gv0++uninits (asz - ssz), tsz+asz)
@@ -650,7 +660,7 @@ Fixpoint _const2GV (TD:TargetData) (M:mem) (gl:GVMap) (c:const)
   : option (GenericValue*typ) := 
 match c with
 | const_zeroinitializer t => 
-  match _zeroconst2GV TD t with
+  match zeroconst2GV TD t with
   | Some gv => Some (gv, t)
   | None => None
   end
@@ -662,7 +672,7 @@ match c with
          match fp with
          | fp_float => Some (val2GV TD (Vfloat f) Mfloat32, typ_floatpoint fp)
          | fp_double => Some (val2GV TD (Vfloat f) Mfloat64, typ_floatpoint fp)
-         | _ => None (*FIXME: not supported 80 and 128 yet. *)
+         | _ => None (* FIXME: not supported 80 and 128 yet. *)
          end
 | const_undef t =>  
          match (getTypeSizeInBits TD t) with
@@ -670,8 +680,14 @@ match c with
          | None => None
          end
 | const_null t => 
-         Some (val2GV TD (Vptr Mem.nullptr (Int.repr 31 0)) (Mint 31), t)
-| const_arr t lc => _list_const_arr2GV TD M gl lc
+         Some (val2GV TD (Vptr Mem.nullptr (Int.repr 31 0)) (Mint 31), 
+               typ_pointer t)
+| const_arr t lc => 
+         match _list_const_arr2GV TD M gl lc with
+         | Some gv => Some (gv, 
+                            typ_array (length (unmake_list_const lc)) t)
+         | _ => None
+         end
 | const_struct lc =>
          match (_list_const_struct2GV TD M gl lc) with
          | None => None
@@ -687,7 +703,7 @@ match c with
          end
 | const_gid t id =>
          match (lookupAL _ gl id) with
-         | Some gv => Some (gv, t)
+         | Some gv => Some (gv, typ_pointer t)
          | None => None
          end
 | const_truncop op c1 t2 =>
@@ -718,22 +734,26 @@ match c with
          | _ => None
          end
 | const_gep ib c1 cs2 =>
-         match Constant.getTyp c1, _const2GV TD M gl c1, Constant.getTyp c with
-         | Some (typ_pointer t1), Some (gv1, _), Some t2 => 
+       match _const2GV TD M gl c1 with
+       | Some (gv1, typ_pointer t1) =>
+         match getConstGEPTyp cs2 (typ_pointer t1) with
+         | Some t2 => 
            match GV2ptr TD (getPointerSize TD) gv1 with
            | Some ptr =>
              match intConsts2Nats TD cs2 with
-             | None => None 
+             | None => Some (uninits 1, t2)
              | Some idxs => 
                match (mgep TD t1 ptr idxs) with
                | Some ptr0 => Some (ptr2GV TD ptr0, t2)
-               | None => None
+               | None => Some (uninits 1, t2)
                end
              end
-           | None => None
+           | None => Some (uninits 1, t2)
            end
-         | _, _, _ => None
+         | _ => None
          end
+       | _ => None
+       end
 | const_select c0 c1 c2 =>
   match _const2GV TD M gl c0, _const2GV TD M gl c1, _const2GV TD M gl c2 with
   | Some (gv0, t0), Some gvt1, Some gvt2 => if isGVZero TD gv0 
@@ -744,8 +764,8 @@ match c with
 | const_icmp cond c1 c2 =>
          match _const2GV TD M gl c1, _const2GV TD M gl c2 with
          | Some (gv1, t1), Some (gv2, _) => 
-           match micmp TD cond t1 gv1 gv2 with
-           | Some gv2 => Some (gv2, typ_int Size.Zero)
+           match micmp TD M cond t1 gv1 gv2 with
+           | Some gv2 => Some (gv2, typ_int Size.One)
            | _ => None
            end
          | _, _ => None
@@ -754,28 +774,32 @@ match c with
          match _const2GV TD M gl c1, _const2GV TD M gl c2 with
          | Some (gv1, typ_floatpoint fp1), Some (gv2, _) => 
            match mfcmp TD cond fp1 gv1 gv2 with
-           | Some gv2 => Some (gv2, typ_int Size.Zero)
+           | Some gv2 => Some (gv2, typ_int Size.One)
            | _ => None
            end
          | _, _ => None
          end
 | const_extractvalue c1 cs2 =>
-         match _const2GV TD M gl c1, Constant.getTyp c with
-         | Some (gv1, t1), Some t2 => 
+       match _const2GV TD M gl c1 with
+       | Some (gv1, t1) =>
+         match getSubTypFromConstIdxs cs2 t1 with 
+         | Some t2 =>
            match extractGenericValue TD t1 gv1 cs2 with
            | Some gv2 => Some (gv2, t2)
            | _ => None
            end
-         | _, _ => None
+         | _ => None
          end
+       | _ => None
+       end
 | const_insertvalue c1 c2 cs3 =>
-         match _const2GV TD M gl c1, _const2GV TD M gl c2, Constant.getTyp c with
-         | Some (gv1, t1), Some (gv2, t2), Some t3 => 
+         match _const2GV TD M gl c1, _const2GV TD M gl c2 with
+         | Some (gv1, t1), Some (gv2, t2) => 
            match insertGenericValue TD t1 gv1 cs3 t2 gv2 with
-           | Some gv3 => Some (gv3, t3)
+           | Some gv3 => Some (gv3, t1)
            | _ => None
            end
-         | _, _, _ => None
+         | _, _ => None
          end
 | const_bop op c1 c2 =>
          match _const2GV TD M gl c1, _const2GV TD M gl c2 with
@@ -797,15 +821,15 @@ match c with
          end
 end
 with _list_const_arr2GV (TD:TargetData) (M:mem) (gl:GVMap) (cs:list_const) 
-  : option (GenericValue*typ) := 
+  : option GenericValue := 
 match cs with
-| Nil_list_const => Some (nil, typ_int Size.Zero)
+| Nil_list_const => Some nil
 | Cons_list_const c lc' =>
   match (_list_const_arr2GV TD M gl lc', _const2GV TD M gl c) with
-  | (Some (gv, t), Some (gv0,t0)) =>
+  | (Some gv, Some (gv0, t0)) =>
              match (getTypeStoreSize TD t0, getTypeAllocSize TD t0) with
              | (Some ssz0, Some asz0) => 
-                 Some ((gv++gv0)++uninits (asz0 - ssz0), t0)
+                 Some ((gv++gv0)++uninits (asz0 - ssz0))
              | _ => None 
              end
   | _ => None
@@ -936,7 +960,7 @@ match (la, lg) with
   updateAddAL _ (_initializeFrameValues la' lg' locals) id g
 | ((t, id)::la', nil) => 
   (* FIXME: We should initalize them w.r.t their type size. *)
-  updateAddAL _ (_initializeFrameValues la' nil locals) id (uninits 0%nat)
+  updateAddAL _ (_initializeFrameValues la' nil locals) id gundef
 | _ => locals
 end.
 
@@ -986,7 +1010,7 @@ end
 Definition ICMP (TD:TargetData) (M:mem) (lc gl:GVMap) (c:cond) (t:typ) 
   (v1 v2:value) : option GenericValue :=
 match (getOperandValue TD M v1 lc gl, getOperandValue TD M v2 lc gl) with
-| (Some gv1, Some gv2) => micmp TD c t gv1 gv2
+| (Some gv1, Some gv2) => micmp TD M c t gv1 gv2
 | _ => None
 end.
 
@@ -995,6 +1019,21 @@ Definition FCMP (TD:TargetData) (M:mem) (lc gl:GVMap) (c:fcond)
 match (getOperandValue TD M v1 lc gl, getOperandValue TD M v2 lc gl) with
 | (Some gv1, Some gv2) => mfcmp TD c fp gv1 gv2
 | _ => None
+end.
+
+Definition GEP (TD:TargetData) (t:typ) (ma:GenericValue) 
+  (vidxs:list GenericValue) (inbounds:bool) : option GenericValue :=
+match GV2ptr TD (getPointerSize TD) ma with
+| Some ptr =>
+  match GVs2Nats TD vidxs with
+  | None => Some gundef
+  | Some idxs => 
+    match (mgep TD t ptr idxs) with
+    | Some ptr0 => Some (ptr2GV TD ptr0)
+    | None => Some gundef
+    end
+  end
+| None => Some gundef
 end.
 
 Lemma BOP_inversion : forall TD M lc gl b s v1 v2 gv,
@@ -1109,7 +1148,7 @@ Lemma ICMP_inversion : forall TD M lc gl cond t v1 v2 gv,
   exists gv1, exists gv2,
     getOperandValue TD M v1 lc gl = Some gv1 /\
     getOperandValue TD M v2 lc gl = Some gv2 /\
-    micmp TD cond t gv1 gv2 = Some gv.
+    micmp TD M cond t gv1 gv2 = Some gv.
 Proof.
   intros TD M lc gl cond0 t v1 v2 gv HICMP.
   unfold ICMP in HICMP.
@@ -1117,7 +1156,7 @@ Proof.
   destruct ogv1; try solve [inversion HICMP].
     remember (getOperandValue TD M v2 lc gl) as ogv2.
     destruct ogv2; try solve [inversion HICMP].
-      remember (micmp TD cond0 t g g0) as R.
+      remember (micmp TD M cond0 t g g0) as R.
       destruct R; inversion HICMP; subst.
         exists g. exists g0. auto.
 Qed.
@@ -1140,6 +1179,7 @@ Proof.
         exists g. exists g0. auto.
 Qed.
 
+(*
 Lemma GEP_inversion : forall (TD:TargetData) (t:typ) (ma:GenericValue) 
   (vidxs:list GenericValue) ib mptr0,
   GEP TD t ma vidxs ib = Some mptr0 ->
@@ -1153,12 +1193,15 @@ Proof.
   unfold GEP in H.
   remember (GVs2Nats TD vidxs) as oidxs.
   remember (GV2ptr TD (getPointerSize TD) ma) as R.
-  destruct R; try solve [inversion H; subst].
-  destruct oidxs; try solve [inversion H; subst].
-  remember (mgep TD t v l0) as og.
-  destruct og; inversion H; subst.
-  exists l0. exists v. exists v0. auto.
+  destruct R.
+    destruct oidxs.
+      remember (mgep TD t v l0) as og.
+      destruct og; inversion H; subst.
+        exists l0. exists v. exists v0. auto.
+        exists l0. exists v. exists v0. auto.
+
 Qed.
+*)
 
 Lemma intValues2Nats_inversion : forall l0 lc gl TD M ns0,
   intValues2Nats TD M l0 lc gl = Some ns0 ->
@@ -1219,6 +1262,10 @@ Proof.
     destruct H0;
     rewrite H1; auto |
 
+    apply H with (TD:=TD)(M:=M)(gl1:=gl1)(gl2:=gl2) in H0;
+    destruct H0;
+    rewrite H0; auto |
+
     rewrite H; auto |
 
     assert (J:=H1);
@@ -1235,11 +1282,8 @@ Proof.
 
   ].
 
-  destruct (Constant.getTyp c); auto.
-  destruct t; auto.
-    assert (J:=H1).
-    apply H with (TD:=TD)(M:=M)(gl1:=gl1)(gl2:=gl2) in H1.
-    rewrite H1. auto.
+  apply H with (TD:=TD)(M:=M)(gl1:=gl1)(gl2:=gl2) in H1.
+  rewrite H1. auto.
 
   assert (J:=H2).
   apply H with (TD:=TD)(M:=M)(gl1:=gl1)(gl2:=gl2) in H2.
