src/SoftBound/test.sh
@@ -17,10 +17,11 @@ OC_DIR=../Parser/tvcases/olden-ccured/
 # em3d: removed 'free', since Softbound is not sound with 'free'.
 OC_CASES="bisort bh em3d health mst perimeter power treeadd tsp"
 S95_DIR=../Parser/tvcases/spec95-ccured/
-# 129.compress has floats and functions named like "\01__soc95"
+# 129.compress has floats and functions named like "\01__soc95" and "@^0"
 # In 099.go 130.li 132.ijpeg there are 'switch'
 # ijpeg: undefined reference to `softbound__01___isoc99_sscanf'
-S95_CASES="099.go 129.compress 130.li"
+# 132.ijpeg is slow for SBpass
+S95_CASES="099.go 130.li"
 OPT_FLAG=
 
 for name in $ML_CASES; do 
@@ -54,6 +55,7 @@ for name in $OC_CASES; do
   llvm-link $name"opt.bc" $BC_DIR"/softbound.bc" $BC_DIR"/softbound-wrappers.bc" > test-softbound.bc
   llvm-ld -native -lm -lcrypt test-softbound.bc -o $name".exe"
 done;
+echo -e "bh: \c"; time ./bh.exe;
 echo -e "bisort: \c"; time ./bisort.exe 5000000 0;
 echo -e "em3d: \c"; time ./em3d.exe 30000 300 50;
 echo -e "health: \c"; time ./health.exe 8 250 1;
@@ -74,7 +76,8 @@ done;
 echo -e "099.go: \c"; time ./099.go.exe 100 15;
 echo -e "130.li: \c"; time ./130.li.exe ../Parser/tvcases/spec95-ccured/130.li/src/ref.lsp;
 rm -f input.* output.* opt.* *.exe *.exe.bc bisort* em3d* health* mst* \
-  treeadd* 129.compress* test-softbound.bc 130.li* 099.go*
+  treeadd* 129.compress* test-softbound.bc 130.li* 099.go* tsp* bh* power* \
+  perimeter*
 
 
 
